\begin{enumerate}[label=\thesubsection.\arabic*, ref=\thesubsection.\theenumi]
	\item If $4x + \i\brak{3x-y} = 3 + \i\brak{-6}$, where $x$ and $y$ are real numbers, then find the values of $x$ and $y$.
	\item If $z_1=2-\i,z_2=1+\i,$ find $\abs{\frac{z_1+z_2+1}{z_1-z_2+1}}$.
	\item Find the real numbers $x$ and $y$ if 
		$\brak{x-\i y}\brak{3+5\i}$ is the conjugate of
		$-6-24\i$.
	\item If $\brak{a+\i b}\brak{c+\i d}\brak{e+\i f}\brak{g+\i h}=A + \i B$, then show that
		$$\brak{a^2+b^2}\brak{c^2+d^2}\brak{d^2+f^2}\brak{f^2+h^2}$$.
\end{enumerate}
	Express the following in the form of $a+b\i$
	\begin{enumerate}[label=\thesubsection.\arabic*, ref=\thesubsection.\theenumi,itemsep=1ex,resume*]
			\begin{multicols}{2}
			\item $\brak{-5\i}\brak{\frac{\i}{8}}$
			\item $\brak{-\i}\brak{-2\i}\brak{\frac{\i}{8}}^3$
			\item $\brak{5\i}\brak{-\frac{3\i}{5}}$
			\item $\brak{5-3\i}^3$
		\item $\frac{5-\sqrt{2}\i}{1-\sqrt{2}\i}$
		\item $\i^{-35}$
		\item $\i^{9}+\i^{19}$
		\item $\i^{-39}$
		\item $3(7 + \i7) + \i (7 + \i7)$
		\item $(1 – i) – ( –1 + i6)$
		\item $\brak{\frac{1}{5}+\frac{2\i}{5}}-\brak{4+\frac{5\i}{2}}$
		\item $\sbrak{\brak{\frac{1}{3}+\frac{7\i}{3}}+\brak{4+\frac{\i}{3}}}-
		\brak{\i -\frac{4}{3}}$
\item $\frac{\brak{3 + \i\sqrt{5}}\brak{3 - \i\sqrt{5}}}{\brak{\sqrt{3} + \i\sqrt{2}}-\brak{\sqrt{3} - \i\sqrt{2}}}$
\item $\sbrak{\i^18+\brak{\frac{1}{\i}}^{25}}$
\item $\brak{\frac{1}{1-4\i}-\frac{2}{1+\i}}\brak{\frac{3-4\i}{5+\i}}$
			\end{multicols}
		\end{enumerate}
Find the multiplicative inverse of the following
\begin{enumerate}[label=\thesubsection.\arabic*, ref=\thesubsection.\theenumi,itemsep=1ex,resume*]
			\begin{multicols}{2}
	\item 	$2-3\i$.
	\item 	$4-3\i$.
	\item 	$\sqrt{5}+3\i$.
	\item 	$-\i$.
			\end{multicols}
\end{enumerate}
Find the conjugate of 
\begin{enumerate}[label=\thesubsection.\arabic*, ref=\thesubsection.\theenumi,resume*]
	\item $\frac{\brak{3-2\i}\brak{2+3\i}}{\brak{1+2\i}\brak{2-\i}}$
\end{enumerate}
